wip

crypto/bignum/poly1305/Hacl.MAC.Poly1305_64.fst
@@ -464,6 +464,55 @@ let store128_le mac mac' =
   Hacl.Spec.Bignum.Fmul.lemma_whole_slice (as_seq h mac);
   Seq.lemma_eq_intro (as_seq h mac) (Seq.append (store64_le_spec macl) (store64_le_spec mach))
 
+#set-options "--z3rlimit 20"
+
+inline_for_extraction val poly1305_finish__:
+  log:log_t ->
+  st:poly1305_state ->
+  mac:uint8_p{length mac = 16} ->
+  m:uint8_p ->
+  len:U64.t{U64.v len < pow2 32 /\ U64.v len <= length m} ->
+  key_s:uint8_p{length key_s = 16} ->
+  Stack log_t
+    (requires (fun h -> live_st h st /\ live h mac /\ live h m /\ live h key_s
+      /\ disjoint st.h mac
+      /\ red_44 (as_seq h st.r) /\ red_45 (as_seq h st.h)))
+    (ensures  (fun h0 updated_log h1 -> modifies_1 st.h h0 h1 /\ live_st h0 st /\ live h0 m
+      /\ live h1 st.h /\ live h1 mac /\ live h0 key_s
+      /\ red_44 (as_seq h0 st.r) /\ red_45 (as_seq h0 st.h)
+      /\ red_45 (as_seq h1 st.h)
+      /\ Spec.MkState (as_seq h1 st.r) (as_seq h1 st.h) () == (
+           assert_norm (pow2 64 = 0x10000000000000000);
+           assert_norm (pow2 32 = 0x100000000);
+           let rem' = U64.(len &^ 0xfuL) in
+           assert_norm(pow2 4 - 1 = 0xf);
+           UInt.logand_mask (U64.v len) 4;
+           if U64.(rem' =^ 0uL) then (Spec.MkState (as_seq h0 st.r) (as_seq h0 st.h) ())
+           else poly1305_process_last_block_spec (Spec.MkState (as_seq h0 st.r) (as_seq h0 st.h) ())
+                                                 (Seq.slice (as_seq h0 m) (U64.v len - U64.v rem') (U64.v len)) rem')
+      ))
+#reset-options "--initial_fuel 0 --max_fuel 0 --z3rlimit 20"
+inline_for_extraction let poly1305_finish__ log st mac m len key_s =
+  assert_norm (pow2 64 = 0x10000000000000000);
+  assert_norm (pow2 32 = 0x100000000);
+  let rem' = U64.(len &^ 0xfuL) in
+  assert_norm(pow2 4 - 1 = 0xf);
+  UInt.logand_mask (U64.v len) 4;
+  let h0 = ST.get() in
+  if U64.(rem' =^ 0uL) then ()
+  else (
+    Math.Lemmas.lemma_div_mod (U64.v len) (16);
+    Math.Lemmas.pow2_lt_compat 64 32;
+    Math.Lemmas.modulo_lemma (U64.v len - U64.v rem') (pow2 32);
+    Math.Lemmas.modulo_lemma (U64.v rem') (pow2 32);
+    let start = Int.Cast.uint64_to_uint32 U64.(len -^ rem') in
+    let l = Int.Cast.uint64_to_uint32 rem' in
+    let last_block = sub m start l in
+    cut (as_seq h0 last_block == (Seq.slice (as_seq h0 m) (U64.v len - U64.v rem') (U64.v len)));
+    poly1305_process_last_block st (sub m start l) rem'
+    );
+  ()
+
 
 val poly1305_finish_:
   log:log_t ->
@@ -482,28 +531,32 @@ val poly1305_finish_:
       /\ as_seq h1 mac == poly1305_finish_spec (Spec.MkState (as_seq h0 st.r) (as_seq h0 st.h) ())
                                               (as_seq h0 m) len (as_seq h0 key_s)
       ))
+#reset-options "--initial_fuel 0 --max_fuel 0 --z3rlimit 20"
 let poly1305_finish_ log st mac m len key_s =
-  assert_norm (pow2 64 = 0x10000000000000000);
-  assert_norm (pow2 32 = 0x100000000);
-  let rem' = U64.(len &^ 0xfuL) in
-  assert_norm(pow2 4 - 1 = 0xf);
-  UInt.logand_mask (U64.v len) 4;
-  let h0 = ST.get() in
-  if U64.(rem' =^ 0uL) then ()
-  else (
-    Math.Lemmas.lemma_div_mod (U64.v len) (16);
-    Math.Lemmas.pow2_lt_compat 64 32;
-    Math.Lemmas.modulo_lemma (U64.v len - U64.v rem') (pow2 32);
-    Math.Lemmas.modulo_lemma (U64.v rem') (pow2 32);
-    let start = Int.Cast.uint64_to_uint32 U64.(len -^ rem') in
-    let l = Int.Cast.uint64_to_uint32 rem' in
-    poly1305_process_last_block st (sub m start l) rem'
-    );
-  let h1 = ST.get() in
-  cut (modifies_1 st.h h0 h1);
+  poly1305_finish__ log st mac m len key_s;  
+  (* assert_norm (pow2 64 = 0x10000000000000000); *)
+  (* assert_norm (pow2 32 = 0x100000000); *)
+  (* let rem' = U64.(len &^ 0xfuL) in *)
+  (* assert_norm(pow2 4 - 1 = 0xf); *)
+  (* UInt.logand_mask (U64.v len) 4; *)
+  (* let h0 = ST.get() in *)
+  (* if U64.(rem' =^ 0uL) then () *)
+  (* else ( *)
+  (*   Math.Lemmas.lemma_div_mod (U64.v len) (16); *)
+  (*   Math.Lemmas.pow2_lt_compat 64 32; *)
+  (*   Math.Lemmas.modulo_lemma (U64.v len - U64.v rem') (pow2 32); *)
+  (*   Math.Lemmas.modulo_lemma (U64.v rem') (pow2 32); *)
+  (*   let start = Int.Cast.uint64_to_uint32 U64.(len -^ rem') in *)
+  (*   let l = Int.Cast.uint64_to_uint32 rem' in *)
+  (*   let last_block = sub m start l in *)
+  (*   cut (as_seq h0 last_block == (Seq.slice (as_seq h0 m) (U64.v len - U64.v rem') (U64.v len))); *)
+  (*   poly1305_process_last_block st (sub m start l) rem' *)
+  (*   ); *)
+  (* let h1 = ST.get() in *)
+  (* cut (modifies_1 st.h h0 h1); *)
   poly1305_last_pass st.h;
   let h2 = ST.get() in
-  cut (modifies_1 st.h h0 h2);
+  (* cut (modifies_1 st.h h0 h2); *)
   cut (disjoint st.h mac);
   let kl = load64_le (sub key_s 0ul 8ul) in
   let kh = load64_le (sub key_s 8ul 8ul) in
@@ -518,8 +571,6 @@ let poly1305_finish_ log st mac m len key_s =
   let k'   = limb_to_wide kl   |^ (limb_to_wide kh   <<^ 64ul) in
   let mac' = acc' +%^ k' in  
   store128_le mac mac'
-  (* store64_le (Buffer.sub mac 0ul 8ul) (wide_to_limb mac'); *)
-  (* store64_le (Buffer.sub mac 8ul 8ul) (wide_to_limb (mac' >>^ 64ul)); *)
 
 
 #reset-options "--initial_fuel 0 --max_fuel 0 --z3rlimit 50"
